Tests/Example.lean
@@ -7,7 +7,7 @@ def xPuzzle : Puzzle 3 3 where
   rowClues i := if i.val = 1 then [1] else [1, 1]
   colClues i := if i.val = 1 then [1] else [1, 1]
 
-example : xPuzzle.Solvable := nono
+example : xPuzzle.Outcome := nono
   fill 1 1
   cross 1 2
   fill 1 3
@@ -21,27 +21,27 @@ example : xPuzzle.Solvable := nono
   fill 3 3
   gram
 
-example : xPuzzle.Solvable := nono
+example : xPuzzle.Outcome := nono
   line
   line row
   line col
   line *
   gram
 
-example : xPuzzle.Solvable := nono
+example : xPuzzle.Outcome := nono
   line row *
   line col *
   gram
 
-example : xPuzzle.Solvable := nono
+example : xPuzzle.Outcome := nono
   line **
   gram
 
-example : xPuzzle.Solvable := nono
+example : xPuzzle.Outcome := nono
   line row 1 * row 2
   gram
 
-example : xPuzzle.Solvable := nono line row 1 3 line col 2 row 2 gram
+example : xPuzzle.Outcome := nono line row 1 3 line col 2 row 2 gram
 
 /-- Row 3 initially has the three candidates `■■■××`, `×■■■×`, and `××■■■`. -/
 def overlapPuzzle : Puzzle 3 5 where
@@ -58,7 +58,7 @@ example :
       some [.unknown, .unknown, .filled, .unknown, .unknown] := by
   native_decide
 
-example : overlapPuzzle.Solvable := nono
+example : overlapPuzzle.Outcome := nono
   line row 3 1 2
   line col 1 2 3 4 5
   gram
@@ -68,7 +68,7 @@ def bear : Puzzle 30 30 := nonogram from clues
   rows: [3 3] [5 7 5] [2 12 2] [2 12 2] 18 17 18 [4 6 6] [4 6 6] [3 1 2 5] [5 3 7] [4 3 6] [4 1 1 1 5] [3 5 5] [3 7] [2 2 5] [10 6] [4 6] [4 7] [4 6] [4 7] [7 3 3 2] [9 6 2 2] [2 9 6 3 3] [1 7 14] [1 7 13] [2 8 10] [11 10] [6 13] 10
   cols: 4 [2 2] [2 2] [3 3] 8 [3 6 10] [5 8 11] [2 11 12] [2 5 5 12] [6 1 5 6] [5 1 1 3 6] [7 1 1 2 3] [8 2 1 1 2 2] [8 4 1 2 2] [8 2 1 1 3 3] [8 1 1 8] [9 1 1 8] [6 1 2 7] [6 1 2 7] [7 5 7] [14 6] [2 13 5] [2 15 6] 28 [3 5 13] [7 2] [5 2] [4 3] 7 4
 
-example : bear.Solvable :=
+example : bear.Outcome :=
   nono
   line col 6 7 8 9 17 21 22 23 24 25
   line row *
@@ -82,7 +82,7 @@ def amb2 : Puzzle 2 2 := nonogram from solution
   ×■
   ■×
 
-example : amb2.Solvable :=
+example : amb2.Outcome :=
   nono
   fill 1 1
   line **
@@ -93,7 +93,7 @@ def amb3_Sub : Puzzle 3 3 := nonogram from solution
   ×■×
   ××■
 
-example : amb3_Sub.Solvable :=
+example : amb3_Sub.Outcome :=
   nono
   line **
   fill 2 2
@@ -111,7 +111,7 @@ def uniqueButLineStalled : Puzzle 5 5 := nonogram from solution
   ××■××
   ■■×××
 
-example : uniqueButLineStalled.Solvable :=
+example : uniqueButLineStalled.Outcome :=
   nono
   line **
 
